

Problem 2

Elias Pers
1016828
lin. alg

$$p(\gamma, z, w | x) = \prod_{d=1}^D q(w_d) \prod_{n=1}^N q(z_n) \prod_{d=1}^D q(\gamma_d)$$

$$p(\gamma, z, w, x) = p(x | \gamma, z, w) \cdot \underbrace{p(\gamma, z, w)}_{= p(\gamma) \cdot p(z) \cdot p(w)}$$

$$= p(x | \gamma, z, w) \cdot p(\gamma) \cdot p(z) \cdot p(w)$$

$$\Rightarrow \log(p(\gamma, z, w, x)) = \log(p(x | \gamma, z, w)) + \log(p(\gamma)) + \log(p(z)) + \log(p(w))$$

$$\log p(x | \gamma, z, w) = \sum_{n=1}^N \log \mathcal{N}_D(x_n | w_{z_n}, \text{diag}(\gamma)^{-1})$$

$$\log \mathcal{N}_D(x_n | w_{z_n}, \text{diag}(\gamma)^{-1}) = -\frac{D}{2} \log 2\pi + \frac{1}{2} \log(\det(\text{diag}(\gamma))) - \frac{1}{2} (x_n - w_{z_n})^T \text{diag}(\gamma) (x_n - w_{z_n})$$

$$\Rightarrow \log p(x | \gamma, z, w) = -\frac{ND}{2} \log 2\pi + \frac{N}{2} \log(\det(\text{diag}(\gamma))) + \sum_{n=1}^N \frac{1}{2} \sum_{d=1}^D (x_n - w_{z_n})^T \text{diag}(\gamma) (x_n - w_{z_n})$$

$$\log p(\gamma) = \sum_{d=1}^D \log \text{Gamma}(\gamma_d | a, b)$$

Elias Felle
101682?
cos P116

$$= \sum_{d=1}^D a \log b - \log \Gamma(a) + (a-1) \log \gamma_d - b \gamma_d$$

$$= D(a \log b - \log \Gamma(a)) + \sum_{d=1}^D (a-1) \log \gamma_d - b \gamma_d$$

$$\log p(z) = \sum_{n=1}^N \log \mathcal{N}_k(z_n | 0, I) = \frac{N}{2} \cdot \log(1) = 0$$

$$= -\frac{NK}{2} \log 2\pi + \frac{N}{2} \log(\det(I))$$

$$- \frac{1}{2} \sum_{n=1}^N (z_n - 0)^T \cdot I (z_n - 0)$$

$$= -\frac{NK}{2} \log 2\pi - \frac{1}{2} \sum_{n=1}^N z_n^T I z_n$$

$$\log p(w) = \sum_{d=1}^D \log \mathcal{N}_k(w_d | 0, \alpha I) \quad I \in \mathbb{R}^{K \times K}$$

$$= -\frac{DK}{2} \log(2\pi) + \frac{D}{2} \log(\det(\alpha I))$$

$\underbrace{\det(\alpha I)}_{= \alpha^K}$

$$- \frac{1}{2} \sum_{d=1}^D w_d^T (\alpha I) w_d$$

$$= -\frac{DK}{2} \log 2\pi + \frac{DK}{2} \log \alpha$$

$$- \frac{1}{2\alpha} \sum_{d=1}^D w_d^T w_d$$

$$\Rightarrow \log p(\gamma, z, w, x)$$

$$= -\frac{ND}{2} \log 2\pi + \frac{N}{2} \log \det(\text{diag}(\gamma)) - \frac{1}{2} \sum_{n=1}^N (x_n - w_{z_n})^T \text{diag}(\gamma) (x_n - w_{z_n})$$

$$+ D(a \log b - \log \Gamma(a)) + \sum_{d=1}^D (a-1) \log \gamma_d - b \gamma_d$$

$$- \frac{NK}{2} \log 2\pi - \frac{1}{2} \sum_{n=1}^N z_n^T z_n$$

$$- \frac{NK}{2} \log 2\pi + \frac{NK}{2} \log \alpha - \frac{1}{2\alpha} \sum_{d=1}^D w_d^T w_d \quad \checkmark$$

part 2

only those terms which depend on z denoted by:

$$\log p_z(\gamma | \log q(z)) = -\frac{1}{2} \sum_{n=1}^N (x_n - w_{z_n})^T \text{diag}(\gamma) (x_n - w_{z_n}) - \frac{1}{2} \sum_{n=1}^N z_n^T z_n$$

$$= -\sum_{n=1}^N \left[\frac{1}{2} (x_n - w_{z_n})^T \text{diag}(\gamma) (x_n - w_{z_n}) - \frac{1}{2} z_n^T z_n \right]$$

lets look at the summands:

$$\frac{1}{2} (x_n - w_{z_n})^T \text{diag}(\gamma) (x_n - w_{z_n}) - \frac{1}{2} z_n^T z_n$$

$$= \frac{1}{2} x_n^T \text{diag}(\gamma) x_n - x_n^T \text{diag}(\gamma) w_{z_n} - \frac{1}{2} z_n^T w_{z_n}^T \text{diag}(\gamma) w_{z_n} - \frac{1}{2} z_n^T z_n$$

discard since
does not depend on z

$$= \frac{1}{2} \mathbf{z}_n^T \underbrace{(W^T \text{diag}(\gamma) W + I)}_A \mathbf{z}_n + \underbrace{\mathbf{x}_n^T \text{diag}(\gamma) W}_{=b^T} \mathbf{z}_n$$

$$\Rightarrow -\frac{1}{2} \mathbf{z}_n^T A \mathbf{z}_n + b^T \mathbf{z}_n$$

apply the completing square technique since
indeed $A^T = A$

$$\Rightarrow -\frac{1}{2} \mathbf{z}_n^T A \mathbf{z}_n + b^T \mathbf{z}_n = -\frac{1}{2} (\mathbf{z}_n - A^{-1}b)^T A (\mathbf{z}_n - A^{-1}b) - \frac{1}{2} b^T A^{-1} b$$

does not depend on \mathbf{z}
 \Rightarrow discard

$$\Rightarrow \log p_{\mathbf{z}}(\log, \mathbf{z}) q(\mathbf{z}) = \sum_{n=1}^N -\frac{1}{2} (\mathbf{z}_n - A^{-1}b)^T A (\mathbf{z}_n - A^{-1}b)$$

where $A = W^T \text{diag}(\gamma) W + I$; $b = W^T \text{diag}(\gamma) \mathbf{x}_n$

now let's look at

$$\log q(\mathbf{z}_n) = -\frac{1}{2} (\mathbf{z}_n - A^{-1}b)^T A (\mathbf{z}_n - A^{-1}b)$$

we notice that this is the form of a normal distribution. The covariance matrix is A^{-1} and the mean is $A^{-1}b$.

$$\Rightarrow q(\mathbf{z}_n) \sim \mathcal{N}_K(A^{-1}b, A^{-1})$$

but since now we need to replace γ and W with their expectations since we assumed that they were given
(sorry for the shitty notation)

$$\Rightarrow A = E_{w, \gamma} [W^T \text{diag}(\gamma) W + I], \quad b = E_{w, \gamma} [W^T \text{diag}(\gamma) x_n]$$

$$A = E_{w, \gamma} [W^T \text{diag}(\gamma) W] + I$$

using the hint

$$= E_{w, \gamma} \left[\sum_{d=1}^D \gamma_d w_d w_d^T \right] + I \quad \text{linearity}$$

$$= E_{\gamma} \sum_{d=1}^D E_{w, \gamma} [\gamma_d w_d w_d^T] + I \quad \text{independence assumption between } \gamma \text{ and } W$$

$$= I + \sum_{d=1}^D \underbrace{E_{\gamma} [\gamma_d]}_{\langle \gamma_d \rangle} \underbrace{E_w [w_d w_d^T]}_{\langle w_d w_d^T \rangle} + I$$

$$= I + \sum_{d=1}^D \langle \gamma_d \rangle \cdot \langle w_d w_d^T \rangle$$

$$\Rightarrow A^{-1} = \left(I + \sum_{d=1}^D \langle \gamma_d \rangle \cdot \langle w_d w_d^T \rangle \right)^{-1} \quad \text{Covariance matrix}$$

Elias Pele
1016828
CU Pele

now the mean similarly, independent "constant"

$$b = E_{w, \gamma} [W^T \text{diag}(\gamma) x_n] = E_{w, \gamma} [W^T \text{diag}(\gamma)] x_n$$

$$= \underbrace{E_w [W^T]}_{\langle W^T \rangle} \cdot \underbrace{E_{\gamma} [\text{diag}(\gamma)]}_{\text{diag}(\langle \gamma \rangle)} x_n$$

$$= \langle W^T \rangle \text{diag}(\langle \gamma \rangle) x_n \Rightarrow A^{-1} b = A^{-1} \langle W^T \rangle \text{diag}(\langle \gamma \rangle) x_n$$

via independence assumption

thus we have shown that the update factor is equal to:

$$q(z_n) = \mathcal{N}_K(M_n, K_n)$$

where $K_n = A^{-1} = \left(I + \sum_{d=1}^D \langle \gamma_d \rangle \langle w_d w_d^T \rangle \right)^{-1}$

$$M_n = A^{-1} b = K_n \langle W^T \rangle \text{diag}(\langle \gamma \rangle) x_n$$



Elias Pels
1016828
cis 249